Update build instructions, add some definitions
The instructions for downloading graphs and building the widgets are now in README.

Added a few definitions about paths in a graph, like:
- longest path
- shortest path
- etc.

Convert/graph.py
@@ -1,0 +1,35 @@
+import json
+from typing import List, Set, Dict, Any
+
+class Graph():
+    """An object representing a single HoG graph"""
+    HoG_id : int
+    vertex_size : int
+    edges : Set[List[int]]
+    hamiltonianPath : List[int]
+
+    def __init__(self, id : str, data : json):
+        self.HoG_id = int(id)
+        adjacency = Graph._parse_adjacency_list(data['adjacencyList'])
+        self.vertex_size = len(adjacency)
+        self.edges = set(Graph._to_edge(int(u), int(v)) for u in adjacency for v in adjacency[u])
+        self.hamiltonianPath = None
+        
+    @staticmethod
+    def _to_edge(fst, snd):
+        return (min(fst, snd), max(fst, snd))
+        
+    @staticmethod
+    def _parse_adjacency_list(adjList) -> Dict[int, Set[int]]:
+        """Return dictionary mapping each vertex to the set of its neighbors."""
+        adjacency : Dict[int, Set[int]]= {}
+        for (i,nbhd) in enumerate(adjList):
+            adjacency[i] = set(nbhd)    
+        return adjacency
+
+    def to_json(self):
+        return {
+            "HoGId" : self.HoG_id,
+            "vertexSize" : self.vertex_size,
+            "edges" : sorted(list(self.edges)),
+        }
