LeanHoG/Invariants/Hamiltonicity/Definition.lean
@@ -88,31 +88,27 @@ end HamiltonianPath
 @[simp] def Cycle.isHamiltonian {g : Graph} {u : g.vertex} (c : Cycle g u) : Bool :=
   ∀ (v : g.vertex), List.contains c.cycle.vertices v
 
-class HamiltonianCycle (g : Graph) (u : g.vertex) where
+class HamiltonianCycle (g : Graph)  where
+  u : g.vertex
   cycle : Cycle g u
   isHamiltonian : cycle.isHamiltonian = true
 
-instance {g : Graph} {u : g.vertex} : Repr (HamiltonianCycle g u) where
+instance {g : Graph} : Repr (HamiltonianCycle g) where
   reprPrec p n := reprPrec p.cycle n
 
-instance {g : Graph} : Repr ((u : g.vertex ) ×' HamiltonianCycle g u) where
+instance {g : Graph} : Repr (HamiltonianCycle g) where
   reprPrec p n := reprPrec p.2.cycle n
 
 @[simp] def Graph.isHamiltonian (g : Graph) : Prop :=
   ∃ (u : g.vertex) (c : Cycle g u), c.isHamiltonian
 
-class HamiltonianGraph (g : Graph) where
-  u : g.vertex
-  cycle : Cycle g u
-  isHamiltonian : cycle.isHamiltonian = true
-
 @[simp] def Graph.isNonHamiltonian (g : Graph) : Prop := ¬ g.isHamiltonian
 
-@[simp] def Graph.isNonHamiltonian' {g : Graph} : Prop := ∀ (u : g.vertex) (c : Cycle g u), ¬c.isHamiltonian
+@[simp] def Graph.isNonHamiltonian' {g : Graph} : Prop :=
+  ∀ (u : g.vertex) (c : Cycle g u), ¬c.isHamiltonian
 
 theorem equivNonHamiltonianDefs (g : Graph) :
   g.isNonHamiltonian ↔ g.isNonHamiltonian' :=
   by simp
-
 
 end LeanHoG
