LeanHoG/Invariants/Hamiltonicity/Tracability.lean
@@ -1,0 +1,15 @@
+import LeanHoG.Walk
+import LeanHoG.Invariants.Hamiltonicity.Definition
+
+namespace LeanHoG
+
+def Graph.isTreacable (G : Graph) : Prop :=
+  ∃ (u : G.vertex) (c : Cycle G u), c.isHamiltonian
+
+lemma hamiltonian_is_traceable {G : Graph} :
+  G.isHamiltonian → G.isTreacable := by
+  intro h
+  let ⟨u, c, hyp⟩ := h
+  sorry
+
+end LeanHoG
