LeanHoG/Invariants/Independence/Definition.lean
@@ -1,0 +1,14 @@
+
+import LeanHoG.Graph
+
+namespace LeanHoG
+
+def isIndependentVertexSet {G : Graph} (S : Finset G.vertex) : Prop :=
+  ∀ (u v : G.vertex), u ∈ S ∧ v ∈ S → ¬ G.adjacent u v
+
+def isMaximumIndependentVertexSet {G : Graph} (S : Finset G.vertex)
+  (_ : isIndependentVertexSet S) : Prop :=
+  ∀ (S' : Finset G.vertex), isIndependentVertexSet S' → S'.card ≤ S.card
+
+
+end LeanHoG
