LeanHoG/LoadGraph.lean
@@ -12,7 +12,7 @@ import LeanHoG.Invariants.Hamiltonicity.SatEncoding
 
 namespace LeanHoG
 
-open Qq LeanSAT Lean Meta
+open Qq LeanSAT Lean Meta Elab Command
 
 /-- Lifting from exception monad to the Elab.Command monad -/
 def liftExcept {α : Type} {m} [Monad m] [Lean.MonadError m] : Except String α → m α
@@ -25,60 +25,60 @@ def certificateName (graphName: Lean.Name) (certName: String) : Lean.Name :=
 
 instance : Solver IO := (Solver.Impl.DimacsCommand "kissat")
 
-/-- A special command for loading a graph -/
-elab "load_graph" graphName:ident fileName:str tryHam:(" tryHam ")? : command => unsafe do
-  let graphName := graphName.getId
-  let gapData ← loadGAPData fileName.getString
-  have graphQ := graphOfData gapData.graph
-  -- load the graph
-  Lean.Elab.Command.liftCoreM <| Lean.addAndCompile <| .defnDecl {
-    name := graphName
-    levelParams := []
-    type := q(Graph)
-    value := q($graphQ)
-    hints := .regular 0
-    safety := .safe
-  }
-  Lean.setReducibleAttribute graphName
-  have graph : Q(Graph) := Lean.mkConst graphName []
+syntax (name := loadGraph) "load_graph" ident str (" tryHam ")? : command
 
-  -- load the connectivity certificate, if present
-  match gapData.connectivityData? with
-  | .none => pure ()
-  | .some data =>
-    let connectivityCertificateName := certificateName graphName "connectivityCertificateI"
-    let connectivityCertificateQ : Q(ConnectivityCertificate $graph) := connectivityCertificateOfData graph data
+@[command_elab loadGraph]
+unsafe def loadGraphImpl : CommandElab
+  | `(load_graph $graphName $fileName tryHam ) => do
+    let graphName := graphName.getId
+    let gapData ← loadGAPData fileName.getString
+    have graphQ := graphOfData gapData.graph
+    -- load the graph
     Lean.Elab.Command.liftCoreM <| Lean.addAndCompile <| .defnDecl {
-      name := connectivityCertificateName
+      name := graphName
       levelParams := []
-      type := q(ConnectivityCertificate $graph)
-      value := connectivityCertificateQ
+      type := q(Graph)
+      value := q($graphQ)
       hints := .regular 0
       safety := .safe
     }
-    Lean.Elab.Command.liftTermElabM <| Lean.Meta.addInstance connectivityCertificateName .scoped 42
+    Lean.setReducibleAttribute graphName
+    have graph : Q(Graph) := Lean.mkConst graphName []
 
-  -- load the disconnectivity certificate, if present
-  match gapData.disconnectivityData? with
-  | .none => pure ()
-  | .some data =>
-    let disconnectivityCertificateName := certificateName graphName "disconnectivityCertificateI"
-    let disconnectivityCertificateQ : Q(DisconnectivityCertificate $graph) := disconnectivityCertificateOfData graph data
-    Lean.Elab.Command.liftCoreM <| Lean.addAndCompile <| .defnDecl {
-      name := disconnectivityCertificateName
-      levelParams := []
-      type := q(DisconnectivityCertificate $graph)
-      value := disconnectivityCertificateQ
-      hints := .regular 0
-      safety := .safe
-    }
-    Lean.Elab.Command.liftTermElabM <| Lean.Meta.addInstance disconnectivityCertificateName .scoped 42
+    -- load the connectivity certificate, if present
+    match gapData.connectivityData? with
+    | .none => pure ()
+    | .some data =>
+      let connectivityCertificateName := certificateName graphName "connectivityCertificateI"
+      let connectivityCertificateQ : Q(ConnectivityCertificate $graph) := connectivityCertificateOfData graph data
+      Lean.Elab.Command.liftCoreM <| Lean.addAndCompile <| .defnDecl {
+        name := connectivityCertificateName
+        levelParams := []
+        type := q(ConnectivityCertificate $graph)
+        value := connectivityCertificateQ
+        hints := .regular 0
+        safety := .safe
+      }
+      Lean.Elab.Command.liftTermElabM <| Lean.Meta.addInstance connectivityCertificateName .scoped 42
 
-  match gapData.pathData? with
-  | .none =>
-    match tryHam with
-    | none => pure ()
-    | some _ =>
+    -- load the disconnectivity certificate, if present
+    match gapData.disconnectivityData? with
+    | .none => pure ()
+    | .some data =>
+      let disconnectivityCertificateName := certificateName graphName "disconnectivityCertificateI"
+      let disconnectivityCertificateQ : Q(DisconnectivityCertificate $graph) := disconnectivityCertificateOfData graph data
+      Lean.Elab.Command.liftCoreM <| Lean.addAndCompile <| .defnDecl {
+        name := disconnectivityCertificateName
+        levelParams := []
+        type := q(DisconnectivityCertificate $graph)
+        value := disconnectivityCertificateQ
+        hints := .regular 0
+        safety := .safe
+      }
+      Lean.Elab.Command.liftTermElabM <| Lean.Meta.addInstance disconnectivityCertificateName .scoped 42
+
+    match gapData.pathData? with
+    | .none =>
       let g ← Elab.Command.liftTermElabM (evalExpr Graph q(Graph) graph)
       let mbHp ← tryFindHamiltonianPath g
       match mbHp with
@@ -96,19 +96,83 @@ elab "load_graph" graphName:ident fileName:str tryHam:(" tryHam ")? : command =>
           safety := .safe
         }
         Lean.Elab.Command.liftTermElabM <| Lean.Meta.addInstance hamiltonianPathName .scoped 42
-  | .some data =>
-    let hamiltonianPathName := certificateName graphName "hamiltonianPath"
-    let hpQ := hamiltonianPathOfData graph data
+    | .some data =>
+      let hamiltonianPathName := certificateName graphName "hamiltonianPath"
+      let hpQ := hamiltonianPathOfData graph data
+      Lean.Elab.Command.liftCoreM <| Lean.addAndCompile <| .defnDecl {
+        name := hamiltonianPathName
+        levelParams := []
+        type := q(HamiltonianPath $graph)
+        value := hpQ
+        hints := .regular 0
+        safety := .safe
+      }
+      Lean.Elab.Command.liftTermElabM <| Lean.Meta.addInstance hamiltonianPathName .scoped 42
+
+  | `(load_graph $graphName $fileName) => do
+    let graphName := graphName.getId
+    let gapData ← loadGAPData fileName.getString
+    have graphQ := graphOfData gapData.graph
+    -- load the graph
     Lean.Elab.Command.liftCoreM <| Lean.addAndCompile <| .defnDecl {
-      name := hamiltonianPathName
+      name := graphName
       levelParams := []
-      type := q(HamiltonianPath $graph)
-      value := hpQ
+      type := q(Graph)
+      value := q($graphQ)
       hints := .regular 0
       safety := .safe
     }
-    Lean.Elab.Command.liftTermElabM <| Lean.Meta.addInstance hamiltonianPathName .scoped 42
+    Lean.setReducibleAttribute graphName
+    have graph : Q(Graph) := Lean.mkConst graphName []
 
+    -- load the connectivity certificate, if present
+    match gapData.connectivityData? with
+    | .none => pure ()
+    | .some data =>
+      let connectivityCertificateName := certificateName graphName "connectivityCertificateI"
+      let connectivityCertificateQ : Q(ConnectivityCertificate $graph) := connectivityCertificateOfData graph data
+      Lean.Elab.Command.liftCoreM <| Lean.addAndCompile <| .defnDecl {
+        name := connectivityCertificateName
+        levelParams := []
+        type := q(ConnectivityCertificate $graph)
+        value := connectivityCertificateQ
+        hints := .regular 0
+        safety := .safe
+      }
+      Lean.Elab.Command.liftTermElabM <| Lean.Meta.addInstance connectivityCertificateName .scoped 42
 
+    -- load the disconnectivity certificate, if present
+    match gapData.disconnectivityData? with
+    | .none => pure ()
+    | .some data =>
+      let disconnectivityCertificateName := certificateName graphName "disconnectivityCertificateI"
+      let disconnectivityCertificateQ : Q(DisconnectivityCertificate $graph) := disconnectivityCertificateOfData graph data
+      Lean.Elab.Command.liftCoreM <| Lean.addAndCompile <| .defnDecl {
+        name := disconnectivityCertificateName
+        levelParams := []
+        type := q(DisconnectivityCertificate $graph)
+        value := disconnectivityCertificateQ
+        hints := .regular 0
+        safety := .safe
+      }
+      Lean.Elab.Command.liftTermElabM <| Lean.Meta.addInstance disconnectivityCertificateName .scoped 42
+
+    match gapData.pathData? with
+    | .none =>
+      pure ()
+    | .some data =>
+      let hamiltonianPathName := certificateName graphName "hamiltonianPath"
+      let hpQ := hamiltonianPathOfData graph data
+      Lean.Elab.Command.liftCoreM <| Lean.addAndCompile <| .defnDecl {
+        name := hamiltonianPathName
+        levelParams := []
+        type := q(HamiltonianPath $graph)
+        value := hpQ
+        hints := .regular 0
+        safety := .safe
+      }
+      Lean.Elab.Command.liftTermElabM <| Lean.Meta.addInstance hamiltonianPathName .scoped 42
+
+  | _ => throwUnsupportedSyntax
 
 end LeanHoG
