js/Build.lean
@@ -1,0 +1,16 @@
+def main : IO Unit := do
+  let exitCode ← IO.Process.spawn {
+    cwd := "js"
+    cmd := "npm"
+    args := #["install", "--silent", "--no-progress"]
+  } >>= (·.wait)
+  if exitCode ≠ 0 then
+    IO.eprintln s!"failed install npm packages"
+
+  let exitCode ← IO.Process.spawn {
+    cwd := "js"
+    cmd := "npm"
+    args := #["run", "build"]
+  } >>= (·.wait)
+  if exitCode ≠ 0 then
+    IO.eprintln s!"failed to run npm build"
