lakefile.lean
@@ -13,3 +13,20 @@ require «lean-sat» from git
 
 @[default_target]
 lean_lib LeanHoG
+
+lean_lib Convert
+lean_lib js
+
+lean_exe get_graphs where
+  root := `Convert.GetGraphs
+
+lean_exe build_widgets where
+  root := `js.Build
+
+post_update pkg do
+  let exitCode ← IO.Process.spawn {
+    cmd := "lake"
+    args := #["exe", "build_widgets"]
+  } >>= (·.wait)
+  if exitCode ≠ 0 then
+    logError s!"{pkg.name}: failed to build widgets"
